Actual Action trait definition

TestModels/dafny-dependencies/StandardLibrary/src/Actions.dfy
@@ -1,36 +1,265 @@
 
 include "../../libraries/src/Wrappers.dfy"
 
-module StandardLibrary.Actions {
+include "Frames.dfy"
+include "GenericAction.dfy"
+include "DecreasesClauses.dfy"
+include "DynamicArray.dfy"
+
+module {:options "--function-syntax:4"} Std.Actions {
 
   import opened Wrappers
+  import opened Frames
+  import opened GenericActions
+  import opened Termination
+  import opened DynamicArray
 
-  // TODO: Add to actual Actions library:
-  // useful pattern to add an Action<Command, Result> facade
-  // to a set of methods that participate in a protocol.
-  // Then you have a history that ties the behavior
-  // of the methods together,
-  // supporting constraints on the order of calls etc.
-  trait {:termination false} Action<T, R> {
-    // ghost var history: seq<(T, R)>
+  // TODO: Documentation, especially overall design
+  trait {:termination false} Action<T, R> extends GenericAction<T, R>, Validatable {
 
-    // predicate Consumes(history: seq<(T, R)>, next: T)
-    // predicate Produces(history: seq<(T, R)>)
-    var Repr: set<object>
+    ghost var history: seq<(T, R)>
 
-    method Call(t: T) returns (r: R)
-      modifies Repr
-      // requires Consumes(history, t)
+    ghost predicate Valid() 
+      reads this, Repr 
+      ensures Valid() ==> this in Repr 
+      ensures Valid() ==> CanProduce(history)
+      decreases height, 0
 
+    // KEY DESIGN POINT: these predicates specifically avoid reading the current
+    // state of the action.
+    // That's so extrisnic properties of an action do NOT depend on their current state.
+    // This is key to ensure that you can prove properties of a given action that
+    // will continue to hold as the Dafny heap changes.
+    // This approach works because Dafny understands that for a given object,
+    // the implementation of CanConsume/CanProduce cannot change over time.
+    //
+    // The downside is that these are then forced to use quantifiers
+    // to talk about all possible states of an action.
+
+    // TODO: Necessary but not sufficient that:
+    // CanConsume(history, nextIn) ==> exists nextOut :: CanProduce(history + [(nextIn, nextOut)])
+    // Does that need to be explicitly part of the spec?
+    ghost predicate CanConsume(history: seq<(T, R)>, next: T)
+      requires CanProduce(history)
+      decreases height
+
+    ghost predicate CanProduce(history: seq<(T, R)>)
+      decreases height
+
+    ghost predicate Requires(t: T)
+      reads Reads(t) 
+    {
+      && Valid()
+      && CanConsume(history, t)
+    }
+    ghost function Reads(t: T): set<object> 
+      reads this
+      ensures this in Reads(t)
+    {
+      {this} + Repr
+    }
+    ghost function Modifies(t: T): set<object> 
+      reads Reads(t)
+    {
+      Repr
+    }
+    ghost function Decreases(t: T): TerminationMetric 
+      reads Reads(t)
+    {
+      NatTerminationMetric(height)
+    }
+    twostate predicate Ensures(t: T, new r: R) 
+      reads Reads(t)
+    {
+      && Valid()
+      && history == old(history) + [(t, r)]
+      && fresh(Repr - old(Repr))
+    }
+
+    // Helpers
+
+    ghost method Update(t: T, r: R)
+      reads `history
+      modifies `history
+      ensures history == old(history) + [(t, r)]
+    {
+      history := history + [(t, r)];
+    }
+
+    ghost function Consumed(): seq<T> 
+      reads this
+    {
+      Inputs(history)
+    }
+
+    ghost function Produced(): seq<R> 
+      reads this
+    {
+      Outputs(history)
+    }
   }
 
-  type SingleUseAction<T, R> = a: Action<T, R>
-    // TODO: Needs indirection or (!new)
-    // TODO: Not quite right, SingleUseAction should be a way of saying
-    // "I will only call this once"
-    // | forall history | a.Produces(history) :: |history| <= 1
-    | true 
-    witness *
+
+  // Dependencies stolen from DafnyStandardLibraries
+  
+  function {:opaque} SeqMap<T, R>(f: (T ~> R), xs: seq<T>): (result: seq<R>)
+    requires forall i :: 0 <= i < |xs| ==> f.requires(xs[i])
+    ensures |result| == |xs|
+    ensures forall i {:trigger result[i]} :: 0 <= i < |xs| ==> result[i] == f(xs[i])
+    reads set i, o | 0 <= i < |xs| && o in f.reads(xs[i]) :: o
+  {
+    if |xs| == 0 then []
+    else [f(xs[0])] + SeqMap(f, xs[1..])
+  }
+
+  function Max(a: int, b: int): int
+  {
+    if a < b
+    then b
+    else a
+  }
+
+  // Common action invariants
+
+  function Inputs<T, R>(history: seq<(T, R)>): seq<T> {
+    SeqMap((e: (T, R)) => e.0, history)
+  }
+
+  function Outputs<T, R>(history: seq<(T, R)>): seq<R> {
+    SeqMap((e: (T, R)) => e.1, history)
+  }
+
+  ghost predicate OnlyProduces<T, R>(i: Action<T, R>, history: seq<(T, R)>, c: R) 
+  {
+    i.CanProduce(history) <==> forall e <- history :: e.1 == c
+  }
+
+  ghost predicate CanConsumeAll<T(!new), R(!new)>(a: Action<T, R>, input: seq<T>) 
+  {
+    forall i | 0 < i < |input| ::
+      var consumed := input[..(i - 1)];
+      var next := input[i];
+      forall history | a.CanProduce(history) && Inputs(history) == consumed :: a.CanConsume(history, next)
+  }
+
+  ghost predicate Terminated<T>(s: seq<T>, c: T, n: nat) {
+    forall i | 0 <= i < |s| :: n <= i <==> s[i] == c
+  }
+
+  lemma TerminatedUndistributes<T>(left: seq<T>, right: seq<T>, c: T, n: nat)
+    requires Terminated(left + right, c, n)
+    ensures Terminated(left, c, n)
+    ensures Terminated(right, c, Max(0, n - |left|))
+  {
+    assert forall i | 0 <= i < |left| :: left[i] == (left + right)[i];
+    assert forall i | 0 <= i < |right| :: right[i] == (left + right)[i + |left|];
+  }
+
+  // TODO: generalize to "EventuallyProducesSequence"?
+  ghost predicate ProducesTerminatedBy<T(!new), R(!new)>(i: Action<T, R>, c: R, limit: nat) {
+    forall history: seq<(T, R)> | i.CanProduce(history) 
+      :: exists n: nat | n <= limit :: Terminated(Outputs(history), c, n)
+  }
+
+  // Class of actions whose precondition doesn't depend on history (probably needs a better name)
+  ghost predicate ContextFree<T(!new), R(!new)>(a: Action<T, R>, p: T -> bool) {
+    forall history, next | a.CanProduce(history)
+      :: a.CanConsume(history, next) <==> p(next)
+  }
+
+  // Aggregators
+
+  type IAggregator<T> = Action<T, ()>
+  type Aggregator<T(!new)> = a: Action<T, bool> | exists limit :: ProducesTerminatedBy(a, false, limit) witness *
+
+  class ArrayAggregator<T> extends Action<T, ()> {
+
+    var storage: DynamicArray<T>
+
+    ghost predicate Valid() 
+      reads this, Repr 
+      ensures Valid() ==> this in Repr 
+      ensures Valid() ==> 
+        && CanProduce(history)
+      decreases height, 0
+    {
+      && this in Repr
+      && storage in Repr
+      && this !in storage.Repr
+      && storage.Repr <= Repr
+      && storage.Valid?()
+      && Consumed() == storage.items
+    }
+
+    constructor() 
+      ensures Valid()
+      ensures fresh(Repr - {this})
+      ensures history == []
+    {
+      var a := new DynamicArray();
+
+      history := [];
+      height := 1;
+      Repr := {this} + {a} + a.Repr;
+      this.storage := a;
+    }
+
+    ghost predicate CanConsume(history: seq<(T, ())>, next: T)
+      decreases height
+    {
+      true
+    }
+    ghost predicate CanProduce(history: seq<(T, ())>)
+      decreases height
+    {
+      true
+    }
+
+    method Invoke(t: T) returns (r: ()) 
+      requires Requires(t)
+      reads Reads(t)
+      modifies Modifies(t)
+      decreases Decreases(t).Ordinal()
+      ensures Ensures(t, r)
+    {
+      storage.Push(t);
+
+      r := ();
+      Update(t, r);
+      Repr := {this} + {storage} + storage.Repr;
+      assert Valid();
+    }
+  }
+
+  method {:rlimit 0} AggregatorExample() {
+    var a := new ArrayAggregator();
+    var _ := a.Invoke(1);
+    var _ := a.Invoke(2);
+    var _ := a.Invoke(3);
+    var _ := a.Invoke(4);
+    var _ := a.Invoke(5);
+    assert a.storage.items == [1, 2, 3, 4, 5];
+  }
+
+  // Other primitives/examples todo:
+  //  * Promise-like single-use Action<T, ()> to capture a value for reading later
+  //  * Eliminate all the (!new) restrictions - look into "older" parameters?
+  //    * How to state the invariant that a constructor as an action creates a new object every time?
+  //      * Lemma that takes produced as input, instead of forall produced?
+  //  * Enumerable ==> defines e.Enumerator()
+  //    * BUT can have infinite containers, probably need IEnumerable as well? (different T for the Action)
+  //  * Expressing that an Action "Eventually produces something" (look at how VMC models this for randomness)
+  //    * IsEnumerator(a) == "a eventually produces None" && "a then only produces None"
+  //    * Build on that to make CrossProduct(enumerable1, enumerable2)
+  //  * Example of adapting an iterator
+  //  * Example of enumerating all possible values of a type (for test generation)
+  //    * Needs to handle infinite types too, hence needs the "eventually produces something" concept
+  //  * Document: useful pattern to add an Action<Command, Result> facade
+  //        to a set of methods that participate in a protocol.
+  //        Then you have a history that ties the behavior
+  //        of the methods together,
+  //        supporting constraints on the order of calls etc.
+
 
   class SeqEnumerator<T> extends Action<(), Option<T>> {
 
@@ -40,7 +269,29 @@ module StandardLibrary.Actions {
       this.values := values;
     }
 
-    method {:verify false} Call(input: ()) returns (value: Option<T>) 
+    ghost predicate Valid() 
+      reads this, Repr 
+      ensures Valid() ==> this in Repr 
+      ensures Valid() ==> CanProduce(history)
+      decreases height, 0
+    {
+      this in Repr
+    }
+    
+    ghost predicate CanConsume(history: seq<((), Option<T>)>, next: ())
+      requires CanProduce(history)
+      decreases height
+    {
+      true
+    }
+
+    ghost predicate CanProduce(history: seq<((), Option<T>)>)
+      decreases height
+    {
+      true
+    }
+
+    method {:verify false} Invoke(input: ()) returns (value: Option<T>) 
       modifies Repr
     {
       if |values| == 0 {
@@ -53,128 +304,50 @@ module StandardLibrary.Actions {
 
   }
 
-  class ComposedAction<T, M, R> extends Action<T, R> {
-
-    const first: Action<T, M>
-    const second: Action<M, R>
-
-    constructor(first: Action<T, M>, second: Action<M, R>) {
-      this.first := first;
-      this.second := second;
-    }
-
-    method {:verify false} Call(input: T) returns (r: R) 
-      modifies Repr
-    {
-      var m := first.Call(input);
-      r := second.Call(m);
-    }
-
-  }
-
-  class FunctionAction<T, R> extends Action<T, R> {
-
-    const f: T -> R
-
-    constructor(f: T -> R) {
-      this.f := f;
-    }
-
-    method {:verify false} Call(input: T) returns (r: R) 
-      modifies Repr
-    {
-      r := f(input);
-    }
-
-  }
-
-  trait {:termination false} Stream<T> {
-    ghost var Repr: set<object>
-
-    method Next() returns (t: Option<T>)
-
-    // TODO: Would be even better if this was a static extern that defaulted
-    // to DefaultForEach(this, a)
-    method ForEach(a: Accumulator<T>)
-  }
-
-  /// Similar to Result, but for delivering a sequence of values instead of just one.
+  // Similar to Result, but for delivering a sequence of values instead of just one.
   // This works better (as opposed to Result<Option<T>, E>)
   // because then a stream that can error is just an Enumerable<Result<T, E>>.
   type StreamEvent<T, E> = Option<Result<T, E>>
 
-
+  type Enumerator<T> = Action<(), Option<T>>
   type Accumulator<T> = Action<T, bool>
 
   method {:verify false} Accept<T>(a: Accumulator<T>, t: T) 
     // requires ConsumesAnything(a)
   {
-    var success := a.Call(t);
+    var success := a.Invoke(t);
     // assert success;
   }
 
-  class Folder<T, R> extends Action<T, bool> {
+  // TODO
+  // class Folder<T, R> extends Action<T, bool> {
 
-    const f: (R, T) -> R
-    var value: R
+  //   const f: (R, T) -> R
+  //   var value: R
 
-    constructor(init: R, f: (R, T) -> R) {
-      this.f := f;
-      this.value := init;
-    }
+  //   constructor(init: R, f: (R, T) -> R) {
+  //     this.f := f;
+  //     this.value := init;
+  //   }
 
-    method {:verify false} Call(t: T) returns (success: bool) {
-      value := f(value, t);
-      return success;
-    }
+  //   method {:verify false} Call(t: T) returns (success: bool) {
+  //     value := f(value, t);
+  //     return success;
+  //   }
 
-  }
+  // }
 
-  method {:verify false} DefaultForEach<T>(s: Stream<T>, a: Accumulator<T>) {
+  method {:verify false} DefaultForEach<T>(s: Enumerator<T>, a: Accumulator<T>) {
     // TODO: Actual Action specs to prove this terminates (iter has to be an Enumerable)
     while (true) {
-      var next := s.Next();
+      var next := s.Invoke(());
       if next == None {
         break;
       }
 
-      var success := a.Call(next.value);
+      var success := a.Invoke(next.value);
       assert success;
     }
-  }
-
-  class SimpleStream<T(0)> extends Stream<T> {
-
-    const iter: Action<(), Option<T>>
-
-    constructor(iter: Action<(), Option<T>>) {
-      this.iter := iter;
-    }
-
-    method {:verify false} Next() returns (t: Option<T>) {
-      t := iter.Call(());
-    }
-
-    method {:verify false} ForEach(a: Accumulator<T>)
-    {
-      DefaultForEach(this, a);
-    }
-
-  }
-
-  class EmptyStream<T> extends Stream<T> {
-
-    constructor() {}
-
-    method {:verify false} Next() returns (t: Option<T>) {
-      t := None;
-    }
-
-    method {:verify false} ForEach(a: Accumulator<T>)
-    {
-      // No-op
-    }
-
   }
 
   // TODO: This is also a Folder([], (x, y) => x + [y])
@@ -186,7 +359,29 @@ module StandardLibrary.Actions {
       values := [];
     }
 
-    method {:verify false} Call(t: T) returns (success: bool) {
+    ghost predicate Valid() 
+      reads this, Repr 
+      ensures Valid() ==> this in Repr 
+      ensures Valid() ==> CanProduce(history)
+      decreases height, 0
+    {
+      this in Repr 
+    }
+
+    ghost predicate CanConsume(history: seq<(T, bool)>, next: T)
+      requires CanProduce(history)
+      decreases height
+    {
+      true
+    }
+
+    ghost predicate CanProduce(history: seq<(T, bool)>)
+      decreases height
+    {
+      true
+    }
+
+    method {:verify false} Invoke(t: T) returns (success: bool) {
       values := values + [t];
     }
 
@@ -199,9 +394,9 @@ module StandardLibrary.Actions {
 
   }
 
-  trait {:termination false} BlockingPipeline<U, T> extends Stream<T> {
+  trait {:termination false} Pipeline<U, T> extends Action<(), Option<T>> {
 
-    const upstream: Stream<U>
+    const upstream: Action<(), Option<U>>
     const buffer: Collector<T>
 
     method {:verify false} Next() returns (t: Option<T>) {
@@ -211,7 +406,7 @@ module StandardLibrary.Actions {
       }
 
       while (|buffer.values| == 0) {
-        var u := upstream.Next();
+        var u := upstream.Invoke(());
         Process(u, buffer);
 
         if u.None? {
@@ -230,7 +425,7 @@ module StandardLibrary.Actions {
     {
       // TODO: Actual Action specs to prove this terminates (iter has to be an Enumerable)
       while (true) {
-        var next := upstream.Next();
+        var next := upstream.Invoke(());
         Process(next, a);
 
         if next == None {
