TestModels/dafny-dependencies/StandardLibrary/src/Index.dfy
@@ -7,5 +7,3 @@ include "./UInt.dfy"
 include "./UTF8.dfy"
 include "./Actions.dfy"
 include "./JavaConversions.dfy"
-
-include "../../dafny/Source/DafnyStandardLibraries/src/Std/Actions/Actions.dfy"
